Remove GenericValueHelper module.

src/Vellvm/opsem.v
@@ -28,40 +28,6 @@ Import LLVMinfra.
 Import LLVMgv.
 Import LLVMtypings.
 
-(* GenericValues represent dynamic values at runtime. We provide
-   different styles of semantics that have different definitions of
-   dynamic values. The following defines their signatures. *)
-Module GenericValueHelper.
-(* instantiate_gvs gv gvs ensures that gvs includes gv. *) 
-(* Definition instantiate_gvs : GenericValue -> GenericValue -> Prop := fun gv1 gv2 => gv1 = gv2. *)
-(* inhabited gvs ensures that gvs is not empty. *)
-(* Definition inhabited : GenericValue -> Prop := fun _ => True. *)
-
-(* Hint Unfold inhabited. *)
-
-(* cgv2gvs cgv t converts the constant cgv to GenericValues w.r.t type t. *)
-(* Definition cgv2gvs : GenericValue -> typ -> GenericValue := LLVMgv.cgv2gv. *)
-(* gv2gvs gv t converts gv to GenericValues in terms of type t. *)
-(* Definition gv2gvs : GenericValue -> typ -> GenericValue := fun gv _ => gv. *)
-(* f is a unary operation of gv, lift_op1 f returns a unary operation of 
-   GenericValues. *)
-
-(* Notation "gv @ gvs" := *)
-(*   (instantiate_gvs gv gvs) (at level 43, right associativity). *)
-(* Notation "$ gv # t $" := (gv2gvs gv t) (at level 41). *)
-
-
-Definition lift_op1 : (GenericValue -> option GenericValue) -> GenericValue -> typ -> option GenericValue :=
-fun (f: GenericValue -> option GenericValue) (gvs1:GenericValue) (ty:typ) => f gvs1.
-(* f is a binary operation of gv, lift_op2 f returns a binary operation of 
-   GenericValues. *)
-Definition lift_op2 : (GenericValue -> GenericValue -> option GenericValue) ->
-  GenericValue -> GenericValue -> typ -> option GenericValue :=
-fun (f: GenericValue -> GenericValue -> option GenericValue)
-  (gvs1 gvs2:GenericValue) (ty: typ) => f gvs1 gvs2.
-(* All values in (cgv2gvs cgv t) are of type size t, match type t, and non-empty.
- *)
-
 Lemma cgv2gvs__getTypeSizeInBits : forall S los nts gv t sz al,
   wf_typ S (los,nts) t ->
   _getTypeSizeInBits_and_Alignment los
@@ -97,124 +63,6 @@ Proof.
   destruct gv; auto.
   eapply cundef_gvs__matches_chunks; eauto.
 Qed.
-
-(* Lemma cgv2gvs__inhabited : forall gv t, inhabited (cgv2gvs gv t). *)
-(* Proof. auto. Qed. *)
-
-(* All values in (gv2gvs gv t) are of type size t, match type t, and non-empty.
- *)
-(* Lemma gv2gvs__getTypeSizeInBits : forall S los nts gv t sz al, *)
-(*   wf_typ S (los,nts) t -> *)
-(*   _getTypeSizeInBits_and_Alignment los *)
-(*     (getTypeSizeInBits_and_Alignment_for_namedts (los,nts) true) true t = *)
-(*       Some (sz, al) -> *)
-(*   Coqlib.nat_of_Z (Coqlib.ZRdiv (Z_of_nat sz) 8) = sizeGenericValue gv -> *)
-(*   sizeGenericValue gv = Coqlib.nat_of_Z (Coqlib.ZRdiv (Z_of_nat sz) 8). *)
-(* Proof. *)
-(*   intros. *)
-(*   intros. auto. *)
-(* Qed. *)
-
-
-(* Lemma gv2gvs__matches_chunks : forall S los nts gv t, *)
-(*   wf_typ S (los,nts) t -> *)
-(*   gv_chunks_match_typ (los, nts) gv t -> *)
-(*   gv_chunks_match_typ (los, nts) gv t. *)
-(* Proof. *)
-(*   intros. auto. *)
-(* Qed. *)
-
-(* Lemma gv2gvs__inhabited : forall gv t, inhabited (gv2gvs gv t). *)
-(* Proof. auto. Qed. *)
-
-(* lift_op1 and lift_op2 preserve inhabitedness, totalness, type size, and 
-   chunks. *)
-(* Lemma lift_op1__inhabited : forall f gvs1 t gvs2 *)
-(*   (H:forall x, exists z, f x = Some z), *)
-(*   inhabited gvs1 -> *)
-(*   lift_op1 f gvs1 t = Some gvs2 -> *)
-(*   inhabited gvs2. *)
-(* Proof. auto. Qed. *)
-
-(* Lemma lift_op2__inhabited : forall f gvs1 gvs2 t gvs3 *)
-(*   (H:forall x y, exists z, f x y = Some z), *)
-(*   inhabited gvs1 -> inhabited gvs2 -> *)
-(*   lift_op2 f gvs1 gvs2 t = Some gvs3 -> *)
-(*   inhabited gvs3. *)
-(* Proof. auto. Qed. *)
-
-Lemma lift_op1__isnt_stuck : forall f gvs1 t
-  (H:forall x, exists z, f x = Some z),
-  exists gvs2, lift_op1 f gvs1 t = Some gvs2.
-Proof. unfold lift_op1. auto. Qed.
-
-Lemma lift_op2__isnt_stuck : forall f gvs1 gvs2 t
-  (H:forall x y, exists z, f x y = Some z),
-  exists gvs3, lift_op2 f gvs1 gvs2 t = Some gvs3.
-Proof. unfold lift_op2. auto. Qed.
-
-Lemma lift_op1__getTypeSizeInBits : forall S los nts f g t sz al gvs,
-  wf_typ S (los,nts) t ->
-  _getTypeSizeInBits_and_Alignment los
-    (getTypeSizeInBits_and_Alignment_for_namedts (los,nts) true) true t =
-      Some (sz, al) ->
-  (forall y, f g = Some y ->
-   sizeGenericValue y = nat_of_Z (ZRdiv (Z_of_nat sz) 8)) ->
-  lift_op1 f g t = Some gvs ->
-  sizeGenericValue gvs = nat_of_Z (ZRdiv (Z_of_nat sz) 8).
-Proof. intros. unfold lift_op1 in H2. eauto. Qed.
-
-Lemma lift_op2__getTypeSizeInBits : forall S los nts f g1 g2 t sz al gvs,
-  wf_typ S (los,nts) t ->
-  _getTypeSizeInBits_and_Alignment los
-    (getTypeSizeInBits_and_Alignment_for_namedts (los,nts) true) true t =
-      Some (sz, al) ->
-  (forall z,
-   f g1 g2 = Some z ->
-   sizeGenericValue z = nat_of_Z (ZRdiv (Z_of_nat sz) 8)) ->
-  lift_op2 f g1 g2 t = Some gvs ->
-  sizeGenericValue gvs = nat_of_Z (ZRdiv (Z_of_nat sz) 8).
-Proof. intros. unfold lift_op2 in H2. eauto. Qed.
-
-Lemma lift_op1__matches_chunks : forall S los nts f g t gvs,
-  wf_typ S (los,nts) t ->
-  (forall y, f g = Some y ->
-   gv_chunks_match_typ (los, nts) y t) ->
-
-
-  lift_op1 f g t = Some gvs ->
-  gv_chunks_match_typ (los, nts) gvs t.
-Proof. intros. unfold lift_op1 in H1. eauto. Qed.
-
-Lemma lift_op2__matches_chunks : forall S los nts f g1 g2 t gvs,
-  wf_typ S (los,nts) t ->
-  (forall z,
-   f g1 g2 = Some z ->
-   gv_chunks_match_typ (los, nts) z t) ->
-  lift_op2 f g1 g2 t = Some gvs ->
-  gv_chunks_match_typ (los, nts) gvs t.
-Proof. intros. unfold lift_op2 in H1. eauto. Qed.
-
-
-(* Inhabited values are not empty. *)
-(* Lemma inhabited_inv : forall gvs, inhabited gvs -> exists gv, gv=gvs. *)
-(* Proof. eauto. Qed. *)
-
-(* gv is in (gv2gvs gv t). *)
-(* Lemma instantiate_gv__gv2gvs : forall gv t, gv = (gv2gvs gv t). *)
-(* Proof. auto. Qed. *)
-
-(* (* If gv's is not undefined, (gv2gvs gv' t) only includes gv'. *) *)
-(* Lemma none_undef2gvs_inv : forall gv' t, *)
-(*   (forall mc, (Vundef, mc)::nil <> gv') -> *)
-(*   (gv2gvs gv' t) = gv'. *)
-(* Proof. *)
-(*   intros. eauto. *)
-(* Qed. *)
-
-Global Opaque lift_op1 lift_op2.
-
-End GenericValueHelper.
 
 Module OpsemAux.
 
@@ -438,15 +286,9 @@ Export OpsemAux.
 Section Opsem.
 
 Definition GVsMap := list (id * GenericValue).
-(* Notation "gv @ gvs" := *)
-(*   (GenericValueHelper.instantiate_gvs gv gvs) (at level 43, right associativity). *)
-(* Notation "$ gv # t $" := (GenericValueHelper.gv2gvs gv t) (at level 41). *)
 
 Definition in_list_gvs (l1 : list GenericValue) (l2 : list GenericValue) : Prop :=
   l1 = l2.
-
-(* Notation "vidxs @@ vidxss" := (in_list_gvs vidxs vidxss) *)
-(*   (at level 43, right associativity). *)
 
 (* Compute the semantic value of a constant. *)
 Definition const2GV (TD:TargetData) (gl:GVMap) (c:const) : option GenericValue :=
@@ -564,7 +406,7 @@ Definition returnUpdateLocals (TD:TargetData) (c':cmd) (Result:value)
   | Some gr =>
       match c' with
       | insn_call id0 false _ ct _ _ _ =>
-           match (GenericValueHelper.lift_op1 (fit_gv TD ct) gr ct) with
+           match (fit_gv TD ct) gr with
            | Some gr' => Some (updateAddAL _ lc' id0 gr')
            | _ => None
            end
@@ -600,7 +442,7 @@ Fixpoint _initializeFrameValues TD (la:args) (lg:list GenericValue) (locals:GVsM
 match (la, lg) with
 | (((t, _), id)::la', g::lg') =>
   match _initializeFrameValues TD la' lg' locals,
-        GenericValueHelper.lift_op1 (fit_gv TD t) g t with
+        (fit_gv TD t) g with
   | Some lc', Some gv => Some (updateAddAL _ lc' id gv)
   | _, _ => None
   end
@@ -621,7 +463,7 @@ Definition BOP (TD:TargetData) (lc:GVsMap) (gl:GVMap) (op:bop) (bsz:sz)
   (v1 v2:value) : option GenericValue :=
 match (getOperandValue TD v1 lc gl, getOperandValue TD v2 lc gl) with
 | (Some gvs1, Some gvs2) =>
-    GenericValueHelper.lift_op2 (mbop TD op bsz) gvs1 gvs2 (typ_int bsz)
+    (mbop TD op bsz) gvs1 gvs2
 | _ => None
 end
 .
@@ -630,7 +472,7 @@ Definition FBOP (TD:TargetData) (lc:GVsMap) (gl:GVMap) (op:fbop) fp
   (v1 v2:value) : option GenericValue :=
 match (getOperandValue TD v1 lc gl, getOperandValue TD v2 lc gl) with
 | (Some gvs1, Some gvs2) =>
-    GenericValueHelper.lift_op2 (mfbop TD op fp) gvs1 gvs2 (typ_floatpoint fp)
+    (mfbop TD op fp) gvs1 gvs2
 | _ => None
 end
 .
@@ -639,7 +481,7 @@ Definition ICMP (TD:TargetData) (lc:GVsMap) (gl:GVMap) c t (v1 v2:value)
   : option GenericValue :=
 match (getOperandValue TD v1 lc gl, getOperandValue TD v2 lc gl) with
 | (Some gvs1, Some gvs2) =>
-    GenericValueHelper.lift_op2 (micmp TD c t) gvs1 gvs2 (typ_int Size.One)
+    (micmp TD c t) gvs1 gvs2
 | _ => None
 end
 .
@@ -648,7 +490,7 @@ Definition FCMP (TD:TargetData) (lc:GVsMap) (gl:GVMap) c fp (v1 v2:value)
   : option GenericValue :=
 match (getOperandValue TD v1 lc gl, getOperandValue TD v2 lc gl) with
 | (Some gvs1, Some gvs2) =>
-    GenericValueHelper.lift_op2 (mfcmp TD c fp) gvs1 gvs2 (typ_int Size.One)
+    (mfcmp TD c fp) gvs1 gvs2
 | _ => None
 end
 .
@@ -656,7 +498,7 @@ end
 Definition CAST (TD:TargetData) (lc:GVsMap) (gl:GVMap) (op:castop)
   (t1:typ) (v1:value) (t2:typ) : option GenericValue:=
 match (getOperandValue TD v1 lc gl) with
-| (Some gvs1) => GenericValueHelper.lift_op1 (mcast TD op t1 t2) gvs1 t2
+| (Some gvs1) => (mcast TD op t1 t2) gvs1
 | _ => None
 end
 .
@@ -664,7 +506,7 @@ end
 Definition TRUNC (TD:TargetData) (lc:GVsMap) (gl:GVMap) (op:truncop)
   (t1:typ) (v1:value) (t2:typ) : option GenericValue:=
 match (getOperandValue TD v1 lc gl) with
-| (Some gvs1) => GenericValueHelper.lift_op1 (mtrunc TD op t1 t2) gvs1 t2
+| (Some gvs1) => (mtrunc TD op t1 t2) gvs1
 | _ => None
 end
 .
@@ -672,14 +514,14 @@ end
 Definition EXT (TD:TargetData) (lc:GVsMap) (gl:GVMap) (op:extop)
   (t1:typ) (v1:value) (t2:typ) : option GenericValue:=
 match (getOperandValue TD v1 lc gl) with
-| (Some gvs1) => GenericValueHelper.lift_op1 (mext TD op t1 t2) gvs1 t2
+| (Some gvs1) => (mext TD op t1 t2) gvs1
 | _ => None
 end
 .
 
 Definition GEP (TD:TargetData) (ty:typ) (mas:GenericValue) (vidxs:list GenericValue)
   (inbounds:bool) ty' : option GenericValue :=
-GenericValueHelper.lift_op1 (gep TD ty vidxs inbounds ty') mas (typ_pointer ty').
+  (gep TD ty vidxs inbounds ty') mas.
 
 Definition extractGenericValue (TD:TargetData) (t:typ) (gvs : GenericValue)
   (cidxs : list const) : option GenericValue :=
@@ -687,7 +529,7 @@ match (intConsts2Nats TD cidxs) with
 | None => None
 | Some idxs =>
   match (mgetoffset TD t idxs) with
-  | Some (o, t') => GenericValueHelper.lift_op1 (mget' TD o t') gvs t'
+  | Some (o, t') => (mget' TD o t') gvs
   | None => None
   end
 end.
@@ -698,7 +540,7 @@ match (intConsts2Nats TD cidxs) with
 | None => None
 | Some idxs =>
   match (mgetoffset TD t idxs) with
-  | Some (o, _) => GenericValueHelper.lift_op2 (mset' TD o t t0) gvs gvs0 t
+  | Some (o, _) => (mset' TD o t t0) gvs gvs0
   | None => None
   end
 end.
@@ -1120,7 +962,7 @@ Definition callUpdateLocals (TD:TargetData) rt (noret:bool) (rid:id)
         | Some Result =>
           match getOperandValue TD Result lc' gl with
           | Some gr =>
-              match (GenericValueHelper.lift_op1 (fit_gv TD rt) gr rt) with
+              match ((fit_gv TD rt) gr) with
               | Some gr' => Some (updateAddAL _ lc rid gr')
               | None => None
               end
